docs/03-formal-verification/easycrypt/games/GameMSHopComposition.ec
@@ -1,4 +1,6 @@
 require import AllCore List.
+require import StdOrder.
+(*---*) import RealOrder.
 require import QssmTypes Algebra Simulator FS TrueClause Comparison ComparisonTypes ComparisonDigests ComparisonPayloads ComparisonCoupling ComparisonCouplingTypes ComparisonCouplingAxioms ComparisonCouplingTheorem ComparisonTheorem.
 require import SourceDistributions SourceTheorem MS LEModel.
 require import GameTypes GameViews GameAdvantage GameMSHopTypes GameMSHopTransitions.
@@ -38,5 +40,30 @@ have H4 := A_MS3b_true_clause_transition x xms s D HS3bbit HS3bcomp HS3bp1 HS3bp
 have H5 := A_MS3c_comparison_transition x xms s D HS3ccomp HS3csim HS3cp1 HS3cp2 HS3cq1 HS3cq2 H3c.
 rewrite /Adv_G0_G1_MS /G_MS_real /G_MS_sim.
 rewrite Htel.
-by smt().
+pose a1 := Adv (G_MS_real x xms s) (G_MS_after_binding x xms s) D.
+pose a2 := Adv (G_MS_after_binding x xms s) (G_MS_after_rom x xms s) D.
+pose a3 := Adv (G_MS_after_rom x xms s) (G_MS_after_bitness x xms s) D.
+pose a4 := Adv (G_MS_after_bitness x xms s) (G_MS_after_comparison x xms s) D.
+pose a5 := Adv (G_MS_after_comparison x xms s) (G_MS_sim x xms s) D.
+have Ha34 : a3 + a4 + a5 <= 0%r.
+  have Ha45 : a4 + a5 <= 0%r by apply (ler_add _ _ _ _ H4 H5).
+  have Hsum : a3 + (a4 + a5) <= 0%r + 0%r by apply (ler_add _ _ _ _ H3 Ha45).
+  have H01 : 0%r + 0%r <= 0%r.
+    have ->: 0%r + 0%r = 0%r by ring.
+    by apply lerr.
+  have Ha34' : a3 + (a4 + a5) <= 0%r by apply (ler_trans _ _ _ Hsum H01).
+  have ->: a3 + a4 + a5 = a3 + (a4 + a5) by ring.
+  exact Ha34'.
+have Ha12345 : a1 + a2 + a3 + a4 + a5 <= a1 + a2.
+  have ->: a1 + a2 + a3 + a4 + a5 = (a1 + a2) + (a3 + a4 + a5) by ring.
+  have Hstep : (a1 + a2) + (a3 + a4 + a5) <= (a1 + a2) + 0%r
+    by apply (ler_add _ _ _ _ (lerr (a1 + a2)) Ha34).
+  have Heq : (a1 + a2) + 0%r = a1 + a2 by ring.
+  have Htail : (a1 + a2) + 0%r <= a1 + a2.
+    rewrite Heq.
+    by apply lerr.
+  by apply (ler_trans _ _ _ Hstep Htail).
+have Ha12 : a1 + a2 <= epsilon_ms_hash_binding + epsilon_ms_rom_programmability
+  by apply (ler_add _ _ _ _ H1 H2).
+apply (ler_trans _ _ _ Ha12345 Ha12).
 qed.
